Syntax and compilation to arrows (#83)

cava/cava/Cava/Arrow/Syntax.v
@@ -1,121 +1,115 @@
-Require Import Coq.Program.Tactics.
-Require Import Coq.Bool.Bool.
-Require Import Coq.Lists.List.
-Require Import Coq.Strings.String.
+Require Export Cava.Arrow.Syntax.Kappa.
+Require Export Cava.Arrow.Syntax.Desugared.
+Require Export Cava.Arrow.Syntax.CC.
 
 Require Import Cava.Arrow.Arrow.
 Require Import Cava.BitArithmetic.
 
-Section KappaVars.
-  Variable arr: Arrow.
-
-  Variable var: object -> object -> Type.
-
-  Inductive kappa : object -> object -> Type :=
-  | Var : forall x y, var x y -> kappa x y
-  | Abs : forall x y z, (var unit x -> kappa y z) -> kappa (x**y) z
-  | App : forall x y z, kappa (x**y) z -> kappa unit x -> kappa y z
-  | Arr : forall x y, morphism x y -> kappa x y
-  | Comp : forall x y z, kappa y z -> kappa x y -> kappa x z
-  | Let : forall x y z, kappa unit x -> (var unit x -> kappa y z) -> kappa y z
-  .
-End KappaVars.
-
-Arguments Var [arr var x y].
-Arguments Abs [arr var x y z].
-Arguments App [arr var x y z].
-Arguments Arr [arr var x y].
-Arguments Comp [arr var x y z].
-Arguments Let [arr var x y z].
-
-(* custom notation *)
+(* Notations *)
 
 Declare Scope source_scope.
 Declare Custom Entry expr.
-
 Delimit Scope source_scope with source.
 
-Notation "<[ \ x => e ]>" := (Abs (fun x => e)) (at level 5, e custom expr at level 1): source_scope.
+Notation "<[ e ]>" := (
+  Desugar _ (fun var => e)
+  ) (at level 1, e custom expr at level 1): source_scope.
+Notation "\ x => e" := (Abs (fun x => e)) (in custom expr at level 1, x constr at level 4, e custom expr at level 4): source_scope.
+
+(* TODO: is this bugged?
+Notation "\ x .. y => e" :=
+  (Abs (fun x =>  ..
+  (Abs (fun y => e)) ..
+  ))
+  (in custom pat at level 1, x constr at level 4, e custom expr at level 4): source_scope. *)
 
 Notation "x y" := (App x y) (in custom expr at level 3, left associativity).
 Notation "~~( x )" := (Arr x) (in custom expr, x constr).
-Notation "~!( x )" := x (in custom expr, x constr).
+Notation "~!( x )" := (Arr (Closure_conversion x)) (in custom expr, x constr).
+(* alternatively *)
+(* Notation "~!( x )" := (kappa_reinject _ (x _)) (in custom expr, x constr). *)
 
 Notation "'let' x = e1 'in' e2" := (Let e1 (fun x => e2)) (in custom expr at level 1, x constr at level 4, e2 at level 5, e1 at level 1).
+Notation "x" := (Var x) (in custom expr, x ident).
+Notation "( x )" := x (in custom expr, x at level 4).
+
+Notation "'fst' e" := (Compose (Arr exl) e) (in custom expr at level 4, e custom expr at level 4).
+Notation "'snd' e" := (Compose (Arr exr) e) (in custom expr at level 4, e custom expr at level 4). 
 
 Notation "# x" := (Arr (constant x)) (in custom expr at level 2, x constr at level 4).
 Notation "#v x" := (Arr (constant_vec _ (nat_to_bitvec_sized _ x))) (in custom expr at level 2, x constr at level 4).
-
-Notation "x" := (Var x) (in custom expr, x ident).
-
-
-Notation "( x )" := x (in custom expr, x at level 4).
-
-(* misc items for testing *)
-
-Definition not' `{Cava}
-  : (bit**unit) ~> bit := exl >>> not_gate.
-
-Definition unsigned_add' `{Cava}
-  {bitsize: nat}
-  : (bitvec bitsize ** bitvec bitsize ** unit) ~> bitvec bitsize :=
-  second exl >>> unsigned_add bitsize bitsize bitsize.
 
 (* test notation *)
 
 Open Scope source_scope.
 
 (* 1. simple constant *)
-
-Definition ex1_plain {cava: Cava} {var}: kappa _ var (bit**unit) bit :=
-Abs (fun x => Arr (constant true)).
-
-Definition ex1_notation {cava: Cava} {var}: kappa _ var (bit**unit) bit :=
+Definition ex1_notation {cava: Cava}: Kappa (bit**unit) bit :=
 <[ \ x => #true ]> .
 
-(* 2. matching types *)
-Definition ex2_plain {cava: Cava} {var} (n:nat) : kappa _ var (bit**unit) bit :=
-match n with
-| O => Abs (fun x => Arr (constant true))
-| S n => Abs (fun x => App (Arr not') (Var x))
-end.
-
-Definition ex2_notation {cava: Cava} {var} (n:nat) : kappa _ var (bit**unit) bit :=
+(* 2. branching on Coq value *)
+Definition ex2_notation {cava: Cava} (n:nat) : Kappa (bit**unit) bit :=
 match n with
 | O => <[ \ x => #true ]>
-| S n => <[ \ x => ~~(not') x ]>
+| S n => <[ \ x => ~~(exl >>> not_gate) x ]>
 end.
 
-(* 3. fixed multiplier, performs addition n times, recursion outside arrow is ciruit duplication *)
-Fixpoint ex3_plain {cava: Cava} {var} {bitsize: nat}
-  (adder: kappa _ var (bitvec bitsize ** bitvec bitsize ** unit) (bitvec bitsize))
-  (n: nat)
-  : kappa _ var (bitvec bitsize**unit) (bitvec bitsize) :=
+(* 3. adder tree *)
+Fixpoint make_obj `{Arrow} o (n:nat) :=
 match n with
-| O => Abs (fun x => Arr (constant_vec bitsize (nat_to_bitvec_sized bitsize 0) ))
-| S n => Abs (fun x : var unit (bitvec bitsize) =>
-    Let (App (ex3_plain adder n) (Var x)) (fun unrolled_circuit =>
-      App (App adder (Var x)) (Var unrolled_circuit)
-    )
-  )
+| O => o
+| S n => make_obj o n ** make_obj o n
 end.
 
-(*
-Fixpoint ex3_notation {cava: Cava} {var} {bitsize: nat}
-  (adder: (bitvec bitsize ** bitvec bitsize ** unit) ~> bitvec bitsize)
-  (n: nat)
-  : (bitvec bitsize**unit) ~> (bitvec bitsize) :=
-*)
-Fixpoint ex3_notation {cava: Cava} {var} {bitsize: nat}
-  (adder: kappa _ var (bitvec bitsize ** bitvec bitsize ** unit) (bitvec bitsize))
-  (n: nat)
-  : kappa _ var (bitvec bitsize**unit) (bitvec bitsize) :=
+Fixpoint tree `{Cava} (A: object)
+  (n: nat) 
+  (f: A**A**unit ~> A)
+  {struct n}
+  : Kappa (make_obj A n ** unit) A :=
 match n with
-| O => <[ \ x => #v 0 ]>
-| S n => <[ \ x =>
-    let unrolled_circuit = ~!( ex3_plain adder n ) x in
-    ~!( adder ) x unrolled_circuit
-    ]>
-(* alternatively: *)
-(* | S n => <[ \ x => ~!( adder ) x ( ~!( ex3_plain adder n ) x ) ]> *)
+| O => <[ \x => x ]>
+| S n' => <[ \x => 
+            let a = ~!(tree A n' f) (fst x) in
+            let b = ~!(tree A n' f) (snd x) in
+
+            ~~(f) a b
+             ]>
 end.
+
+Definition adder_tree `{Cava} 
+  (bitsize: nat)
+  (n: nat)
+  : Kappa (make_obj (bitvec bitsize) n ** unit) (bitvec bitsize) :=
+  tree (bitvec bitsize) n (unassoc >>> exl >>> unsigned_add _ _ _).
+
+Notation "'coerce_variable_environment' b" := (morphism_coerce _ b _)
+  (only printing, at level 0).
+
+Notation "v : 'u' sz" := (constant_vec sz (nat_to_bitvec_sized sz v))
+  (only printing, at level 99, format "'[ ' v : 'u' sz ']'").
+
+Ltac unfold_notation :=
+  repeat (unfold Desugar;
+  unfold desugar;
+  unfold Closure_conversion;
+  unfold closure_conversion;
+  simpl).
+
+Lemma kappa_arrow_lemma_example: 
+  forall (Cava: Cava), 
+  Closure_conversion ex1_notation = (uncancelr >>> first swap >>> assoc >>> exl >>> constant true).
+Proof.
+  intros.
+  unfold ex1_notation.
+  unfold_notation.
+  auto.
+Qed.
+
+Lemma adder_tree_lemma_example: 
+  forall (Cava: Cava), 
+  Closure_conversion (adder_tree 8 3) <> (drop >>> constant_vec _ (nat_to_bitvec_sized _ 0)).
+Proof.
+  intros.
+  unfold ex1_notation.
+  unfold_notation.
+  Admitted.
