cava/cava/Cava/Arrow.v
@@ -2,3 +2,5 @@ Require Export Cava.Arrow.Arrow.
 Require Export Cava.Arrow.Instances.Coq.
 Require Export Cava.Arrow.Instances.Netlist.
 Require Export Cava.Arrow.Instances.Stream.
+
+Require Export Cava.Arrow.Syntax.
