cava/cava/Cava/Arrow/Syntax/Desugared.v
@@ -1,0 +1,61 @@
+Require Import Cava.Arrow.Arrow.
+Require Import Cava.Arrow.Syntax.Kappa.
+
+Reserved Infix "<-->" (at level 90, no associativity).
+Reserved Infix "≅" (at level 90, no associativity).
+Reserved Infix "--->" (at level 90, no associativity).
+
+Section WithArrow.
+  Variable arr: Arrow.
+
+  Section Vars.
+    Variable var: object -> object -> Type.
+
+    (* desugared, currently only let removal *)
+    Inductive kappa : object -> object -> Type :=
+    | DVar : forall x y,   var x y -> kappa x y
+    | DAbs : forall x y z, (var unit x -> kappa y z) -> kappa (x**y) z
+    | DApp : forall x y z, kappa (x**y) z -> kappa unit x -> kappa y z
+    | DCompose : forall x y z, kappa y z -> kappa x y -> kappa x z
+    | DArr : forall x y,   morphism x y -> kappa x y.
+  End Vars.
+
+  Arguments DVar [var x y].
+  Arguments DAbs [var x y z].
+  Arguments DApp [var x y z].
+  Arguments DCompose [var x y z].
+  Arguments DArr [var x y].
+
+  Definition Kappa i o := forall var, @kappa var i o.
+
+  (* currently only desugars let bindings *)
+  Fixpoint desugar {var i o} (e: kappa_sugared var i o) : kappa var i o :=
+  match e with
+  | Var x => DVar x
+  | Abs f => DAbs (fun x => desugar (f x))
+  | App e1 e2 => DApp (desugar e1) (desugar e2)
+  | Compose f g => DCompose (desugar f) (desugar g)
+  | Arr m => DArr m
+  | Let x f => DApp (DAbs (fun x => desugar (f x))) (desugar x)
+  end.
+
+  Definition Desugar {i o} (e: Kappa_sugared i o) : Kappa i o := fun var => desugar (e var).
+
+  Fixpoint kappa_reinject {var i o} (e: kappa var i o) : kappa_sugared var i o :=
+  match e with
+  | DVar x => Var x
+  | DAbs f => Abs (fun x => kappa_reinject (f x))
+  | DApp e1 e2 => App (kappa_reinject e1) (kappa_reinject e2)
+  | DCompose f g => Compose (kappa_reinject f) (kappa_reinject g)
+  | DArr m => Arr m
+  end.
+End WithArrow.
+
+Arguments DVar [arr var x y].
+Arguments DAbs [arr var x y z].
+Arguments DApp [arr var x y z].
+Arguments DCompose [arr var x y z].
+Arguments DArr [arr var x y].
+
+Arguments kappa [arr].
+Arguments Kappa [arr].
